thys/MFODL_Monitor_Devel/Optimized_Agg_Temporal.thy
@@ -19,16 +19,20 @@ fun delete_maggaux' :: "aggargs \<Rightarrow> event_data option list set \<Right
   "delete_maggaux' args X (Some aux) = (let (v', aux') = delete_maggaux args X aux in
                                        if v' then Some aux' else None)"
 
+fun result_maggaux' :: "aggargs \<Rightarrow> aggaux option \<Rightarrow> event_data option list set option" where
+  "result_maggaux' args None = None" |
+  "result_maggaux' args (Some aux) = Some (result_maggaux args aux)"
+
 fun valid_maggaux' :: "aggargs \<Rightarrow> aggaux option \<Rightarrow> event_data option list set \<Rightarrow> bool" where
   "valid_maggaux' args None X = True" |
   "valid_maggaux' args (Some aux) X = valid_maggaux args aux X"
 
 fun valid_mmasaux :: "args \<Rightarrow> ts \<Rightarrow> mmasaux \<Rightarrow> event_data Monitor.msaux \<Rightarrow> bool" where
   "valid_mmasaux args cur ((nt, gc, maskL, maskR, data_prev, data_in, tuple_in, tuple_since), aggaux) ys =
+   (valid_mmsaux args cur (nt, gc, maskL, maskR, data_prev, data_in, tuple_in, tuple_since) ys \<and>
     (case args_agg args of
-      Some aggargs \<Rightarrow> (valid_mmsaux args cur (nt, gc, maskL, maskR, data_prev, data_in, tuple_in, tuple_since) ys \<and> 
-                      valid_maggaux' aggargs aggaux (Mapping.keys tuple_in)) |
-      None \<Rightarrow> valid_mmsaux args cur (nt, gc, maskL, maskR, data_prev, data_in, tuple_in, tuple_since) ys)"
+      Some aggargs \<Rightarrow> valid_maggaux' aggargs aggaux (Mapping.keys tuple_in) |
+      None \<Rightarrow> True))"
 
 fun init_mmasaux :: "args \<Rightarrow> mmasaux" where
   "init_mmasaux args =  (case args_agg args of
@@ -50,10 +54,10 @@ fun join_mmasaux :: "args \<Rightarrow> event_data table \<Rightarrow> mmasaux \
       None \<Rightarrow> (join_mmsaux args X (t, gc, maskL, maskR, data_prev, data_in, tuple_in, tuple_since), aggaux) |
       Some aggargs \<Rightarrow>
     (let pos = args_pos args in
-    (if maskL = maskR then
-      (let tuple_in' = Mapping.filter (join_filter_cond pos X) tuple_in;
+    (if maskL = maskR then                                
+      (let (tuple_in', to_del) = (Mapping.filter (join_filter_cond pos X) tuple_in, Mapping.keys tuple_in - Mapping.keys (Mapping.filter (join_filter_cond pos X) tuple_in));
       tuple_since = Mapping.filter (join_filter_cond pos X) tuple_since in
-      ((t, gc, maskL, maskR, data_prev, data_in, tuple_in', tuple_since), delete_maggaux' aggargs (Mapping.keys tuple_in - Mapping.keys tuple_in') aggaux))
+      ((t, gc, maskL, maskR, data_prev, data_in, tuple_in', tuple_since), delete_maggaux' aggargs to_del aggaux))
     else if (\<forall>i \<in> set maskL. \<not>i) then
       (let nones = replicate (length maskL) None;
       take_all = (pos \<longleftrightarrow> nones \<in> X); 
@@ -80,8 +84,8 @@ fun shift_end_mmasaux :: "args \<Rightarrow> ts \<Rightarrow> mmasaux \<Rightarr
     (let I = args_ivl args;
     data_prev' = dropWhile_queue (\<lambda>(t, X). \<not> memR I (nt - t)) data_prev;
     (data_in, discard) = takedropWhile_queue (\<lambda>(t, X). \<not> memR I (nt - t)) data_in;
-    (tuple_in, aggaux) = fold (\<lambda>(t, X) (tuple_in, aux). let tuple_in' = Mapping.filter (filter_cond X tuple_in t) tuple_in in
-    (tuple_in', delete_maggaux' aggargs (Mapping.keys tuple_in - Mapping.keys tuple_in') aux)) discard (tuple_in, aggaux) in
+    (tuple_in, aggaux) = fold (\<lambda>(t, X) (tuple_in, aux). let (tuple_in', to_del) = (Mapping.filter (filter_cond X tuple_in t) tuple_in, Mapping.keys tuple_in - Mapping.keys (Mapping.filter (filter_cond X tuple_in t) tuple_in)) in
+    (tuple_in', delete_maggaux' aggargs to_del aux)) discard (tuple_in, aggaux) in
     ((t, gc, maskL, maskR, data_prev', data_in, tuple_in, tuple_since), aggaux)))"
 
 fun add_new_ts_mmasaux' :: "args \<Rightarrow> ts \<Rightarrow> mmasaux \<Rightarrow> mmasaux" where
@@ -108,7 +112,6 @@ fun result_mmasaux :: "args \<Rightarrow> mmasaux \<Rightarrow> event_data table
 
 lemma valid_init_mmasaux: 
   assumes "L \<subseteq> R"
-  and "valid_aggargs n R agg"
   shows "valid_mmasaux (init_args I n L R b agg) 0
   (init_mmasaux (init_args I n L R b agg)) []"
 proof(cases agg)
@@ -116,7 +119,6 @@ proof(cases agg)
   then show ?thesis using valid_init_mmsaux[OF assms(1), of I n b agg] by(simp only:init_args_def init_mmasaux.simps) simp
 next
   case (Some aggargs)
-  then have safe_aggargs: "safe_aggargs aggargs" using assms(2) by(simp add:valid_aggargs_def)
   show ?thesis using Some valid_init_mmsaux[OF assms(1), of I n b agg] 
      valid_init_maggaux[of aggargs] by(cases "type_restr aggargs {}") (auto simp: init_args_def) 
 qed
@@ -161,7 +163,7 @@ proof -
         proof(cases "memL (args_ivl args) 0")
           case True
           then have finite: "finite (rel2 - Mapping.keys tuple_in)" 
-            using new_def some_aggargs Some by(simp del:insert_maggaux.simps split:prod.splits if_splits) 
+            using new_def some_aggargs Some by(simp del:insert_maggaux.simps split:prod.splits if_splits)
           then show ?thesis using True Some some_aggargs new_def valid_msaux' valid_insert_maggaux[OF valid_maggaux finite] split tuple_in_eq
             by(simp del:valid_mmsaux.simps split:prod.splits if_splits)
         next
@@ -238,9 +240,9 @@ proof -
         have *: "join_mmasaux args rel1 ((nt, gc, maskL, maskR, data_prev, data_in, tuple_in, tuple_since), aggaux) = ?temp" 
           using False Some True by simp blast
         have "valid_mmasaux args cur ?temp (map (\<lambda>(t, rel). (t, join rel (args_pos args) rel1)) auxlist)"
-          using valid_msaux' neq True valid_init_maggaux assms(1) some_aggargs sorry
-          (*by(simp del:valid_mmsaux.simps split:if_splits option.splits) (smt (z3) case_prodD)+*)
-        then show ?thesis using * by simp
+          using valid_msaux' neq True valid_init_maggaux assms(1) some_aggargs
+          by(simp del:valid_mmsaux.simps split:if_splits option.splits) 
+        then show ?thesis using * by presburger
       next
         case False
         let ?temp = "let tuple_in' = Mapping.filter (\<lambda>as _. proj_tuple_in_join (args_pos args) maskL as rel1) tuple_in;
@@ -259,7 +261,7 @@ proof -
             some_aggargs Some valid_msaux' neq False mapping_filter_keys_diff[of _ tuple_in, symmetric]
             by(simp del:delete_maggaux.simps valid_mmsaux.simps split:option.splits prod.splits if_splits)
         qed
-        then show ?thesis using * by simp
+        then show ?thesis using * by presburger
       qed
     qed
   qed
@@ -449,7 +451,7 @@ proof -
   next
     case (Some a)
     then show ?thesis using tuple_in_rel assms valid_result_maggaux 
-      by(auto simp del: valid_mmsaux.simps simp add: eval_args_agg_def split:option.splits) 
+      by(auto simp del: valid_mmsaux.simps simp add: eval_args_agg_def split:option.splits)
   qed
 qed
 
@@ -461,6 +463,507 @@ interpretation default_mmasaux: msaux valid_mmasaux init_mmasaux add_new_ts_mmas
   add_new_table_mmasaux result_mmasaux
   using valid_init_mmasaux valid_add_new_ts_mmasaux valid_gc_join_mmasaux valid_add_new_table_mmasaux
     valid_result_mmasaux
+  by unfold_locales (auto simp del: valid_mmasaux.simps split:prod.splits)
+
+type_synonym mmauaux = "event_data mmuaux \<times> aggaux option \<times> event_data table option list"
+
+fun valid_aggaux_list :: "Monitor.args \<Rightarrow> event_data option list set list \<Rightarrow> event_data table option list \<Rightarrow> bool"where
+  "valid_aggaux_list args [] [] = True" |
+  "valid_aggaux_list args (x#xs) (y#ys) = (valid_aggaux_list args xs ys \<and>
+                                          (case y of Some k \<Rightarrow> (k = eval_args_agg args x) |
+                                                     None \<Rightarrow> True))" |
+  "valid_aggaux_list _ _ _ = False"
+
+fun valid_mmauaux' :: "args \<Rightarrow> ts \<Rightarrow> ts \<Rightarrow> mmauaux \<Rightarrow> event_data muaux \<Rightarrow> bool" where
+  "valid_mmauaux' args cur dt ((tp, tss, len, maskL, maskR, a1_map, a2_map, done, done_length), aggaux, done_agg) auxlist 
+ = (valid_mmuaux' args cur dt (tp, tss, len, maskL, maskR, a1_map, a2_map, done, done_length) auxlist \<and>
+  (case args_agg args of
+      Some aggargs \<Rightarrow> (valid_maggaux' aggargs aggaux (Mapping.keys (the (Mapping.lookup a2_map tp))) \<and>
+                      valid_aggaux_list args done done_agg) |
+      None \<Rightarrow> True))"
+
+definition valid_mmauaux :: "args \<Rightarrow> ts \<Rightarrow> mmauaux \<Rightarrow> event_data muaux \<Rightarrow> bool" where
+  "valid_mmauaux args cur = valid_mmauaux' args cur cur"
+
+fun init_mmauaux :: "args \<Rightarrow> mmauaux" where
+  "init_mmauaux args = (init_mmuaux args, (case args_agg args of
+    Some aggargs \<Rightarrow> init_maggaux' aggargs |
+    None \<Rightarrow> None), [])"
+
+fun lin_ts_mmauaux :: "mmauaux \<Rightarrow> ts list" where
+  "lin_ts_mmauaux ((tp, tss, len, maskL, maskR, a1_map, a2_map, done, done_length), auxs, done_agg) =
+    linearize tss"
+
+fun eval_step_mmauaux :: "args \<Rightarrow> mmauaux \<Rightarrow> mmauaux" where
+  "eval_step_mmauaux args ((tp, tss, len, maskL, maskR, a1_map, a2_map, done, done_length), aggaux, done_agg) = 
+  (case safe_hd tss of 
+  (Some ts, tss') \<Rightarrow>
+    (case args_agg args of 
+    None \<Rightarrow> (eval_step_mmuaux args (tp, tss, len, maskL, maskR, a1_map, a2_map, done, done_length), aggaux, done_agg) |
+    Some aggargs \<Rightarrow>
+      (case Mapping.lookup a2_map (tp - len) of 
+      Some m \<Rightarrow> 
+        let T = Mapping.keys m;
+        tss' = tl_queue tss';
+        ts' = case safe_hd tss' of 
+              (Some ts', tss'') \<Rightarrow> ts';
+        m'' =  Mapping.filter (\<lambda> _ tstp. ts_tp_lt (args_ivl args) ts' (tp - len + 1) tstp) m;
+        to_del = Mapping.keys m - Mapping.keys m'';
+        to_ins = case Mapping.lookup a2_map (tp - len + 1) of Some m' \<Rightarrow> m';
+        a2_map = Mapping.update (tp - len + 1)
+          (Mapping.combine (\<lambda>tstp tstp'. max_tstp tstp tstp') m'' to_ins) a2_map;
+        a2_map = Mapping.delete (tp - len) a2_map;
+        agg_result = result_maggaux' aggargs aggaux;
+        aggaux = insert_maggaux' aggargs (Mapping.keys to_ins) (delete_maggaux' aggargs to_del aggaux) in
+        ((tp, tss', len - 1, maskL, maskR, a1_map, a2_map,
+        T # done, done_length + 1), aggaux, agg_result#done_agg))))"
+
+fun shift_mmauaux :: "args \<Rightarrow> ts \<Rightarrow> mmauaux \<Rightarrow> mmauaux" where
+  "shift_mmauaux args nt ((tp, tss, len, maskL, maskR, a1_map, a2_map, done, done_length), auxs, done_agg) =
+    (let tss_list = linearize (takeWhile_queue (\<lambda>t. \<not> memR (args_ivl args) (nt - t)) tss) in
+    foldl (\<lambda>aux _. eval_step_mmauaux args aux) ((tp, tss, len, maskL, maskR,
+      a1_map, a2_map, done, done_length), auxs, done_agg) tss_list)"
+
+fun add_new_mmauaux :: "args \<Rightarrow> event_data table \<Rightarrow> event_data table \<Rightarrow> ts \<Rightarrow> mmauaux \<Rightarrow> mmauaux" where
+  "add_new_mmauaux args rel1 rel2 nt (mmuaux, aggaux, done_agg) =
+    (case args_agg args of 
+     None \<Rightarrow> (add_new_mmuaux args rel1 rel2 nt mmuaux, aggaux, done_agg) |
+     Some aggargs \<Rightarrow>
+    (let ((tp, tss, len, maskL, maskR, a1_map, a2_map, done, done_length), aggaux, done_agg) = shift_mmauaux args nt (mmuaux, aggaux, done_agg);
+    I = args_ivl args; pos = args_pos args;
+    new_tstp = (if memL I 0 then Inr tp else Inl nt);
+    tmp = \<Union>((\<lambda>as. case Mapping.lookup a1_map (proj_tuple maskL as) of None \<Rightarrow>
+      (if \<not>pos then {(tp - len, as)} else {})
+      | Some tp' \<Rightarrow> if pos then {(max (tp - len) tp', as)}
+      else {(max (tp - len) (tp' + 1), as)}) ` rel2) \<union> (if memL I 0 then {tp} \<times> rel2 else {});
+    a2_map' = Mapping.update (tp + 1) Mapping.empty
+      (upd_nested a2_map new_tstp (max_tstp new_tstp) tmp);
+    a1_map = (if pos then Mapping.filter (\<lambda>as _. as \<in> rel1)
+      (upd_set a1_map (\<lambda>_. tp) (rel1 - Mapping.keys a1_map)) else upd_set a1_map (\<lambda>_. tp) rel1);
+    tss = append_queue nt tss in
+    ((tp + 1, tss, len + 1, maskL, maskR, a1_map, a2_map', done, done_length), aggaux, done_agg)))"
+
+fun length_mmauaux :: "args \<Rightarrow> mmauaux \<Rightarrow> nat" where
+  "length_mmauaux args ((tp, tss, len, maskL, maskR, a1_map, a2_map, done, done_length), auxs, done_agg) =
+    len + done_length"
+
+fun eval_mmauaux :: "args \<Rightarrow> ts \<Rightarrow> mmauaux \<Rightarrow> (event_data table list \<times> event_data table option list \<times> mmauaux)" where
+  "eval_mmauaux args nt aux =
+    (let ((tp, tss, len, maskL, maskR, a1_map, a2_map, done, done_length), auxs, done_agg) =
+    shift_mmauaux args nt aux in
+    (rev done, rev done_agg, ((tp, tss, len, maskL, maskR, a1_map, a2_map, [], 0), auxs, [])))"
+
+fun combine_res where
+  "combine_res args [] [] = []" |
+  "combine_res args (x#xs) (y#ys) = (case y of Some k \<Rightarrow> k |
+                                               None \<Rightarrow> eval_args_agg args x)#combine_res args xs ys"
+          
+
+definition "eval_mmauaux' args nt aux = (case eval_mmauaux args nt aux of (res, res_agg, aux') \<Rightarrow>
+    (combine_res args res res_agg, aux'))"
+
+lemma valid_length_mmauaux:
+  assumes "valid_mmauaux args cur (mmaux, auxs, done_agg) auxlist"
+  shows "length_mmauaux args (mmaux, auxs, done_agg) = length auxlist"
+  using assms by (cases mmaux) (auto simp add: valid_mmauaux_def dest: list_all2_lengthD)
+
+lemma valid_init_mmauaux:
+  assumes "L \<subseteq> R" 
+  shows "valid_mmauaux (init_args I n L R b agg) 0 (init_mmauaux (init_args I n L R b agg)) []"
+proof -
+  let ?map = "Mapping.update 0 Mapping.empty Mapping.empty"
+  note valid_mmuaux = valid_init_mmuaux[OF assms, of I n b agg] 
+  show ?thesis 
+  proof (cases "agg")
+    case None
+    then show ?thesis using valid_mmuaux
+      by(simp only:init_args_def init_mmauaux.simps) (simp add: init_mmuaux_def valid_mmauaux_def valid_mmuaux_def) 
+  next
+    case (Some a)
+    then show ?thesis using valid_mmuaux Some valid_init_maggaux[of a]
+      by(simp only:init_args_def init_mmauaux.simps) (auto simp add: Mapping.lookup_update[of 0 Mapping.empty Mapping.empty] simp del: valid_mmuaux'.simps simp add: init_mmuaux_def valid_mmauaux_def valid_mmuaux_def)
+  qed
+qed
+
+lemma valid_eval_step_mmauaux_unfolded:
+  assumes "valid_mmauaux' args cur dt ((tp, tss, len, maskL, maskR, a1_map, a2_map, done, done_length), auxs, done_agg) auxlist"
+    "lin_ts_mmauaux ((tp, tss, len, maskL, maskR, a1_map, a2_map, done, done_length), auxs, done_agg) = ts # tss''" "\<not> memR (args_ivl args) (dt - ts)"
+  shows "valid_mmauaux' args cur dt (eval_step_mmauaux args ((tp, tss, len, maskL, maskR, a1_map, a2_map, done, done_length), auxs, done_agg)) auxlist \<and>
+    lin_ts_mmauaux (eval_step_mmauaux args ((tp, tss, len, maskL, maskR, a1_map, a2_map, done, done_length), auxs, done_agg)) = tss'' \<and>
+    (case eval_step_mmauaux args ((tp, tss, len, maskL, maskR, a1_map, a2_map, done, done_length), auxs, done_agg) of
+    (mmaux', auxs', done_agg') \<Rightarrow> mmaux' = eval_step_mmuaux args (tp, tss, len, maskL, maskR, a1_map, a2_map, done, done_length))"
+proof -
+  let ?muaux = "(tp, tss, len, maskL, maskR, a1_map, a2_map, done, done_length)"
+  obtain tss' where safe_hd_eq: "safe_hd tss = (Some ts, tss')" using assms(2) safe_hd_rep case_optionE by (cases "safe_hd tss") fastforce
+  have a2_map_keys: "Mapping.keys a2_map = {tp - len..tp}"
+    using assms(1) by auto
+  have tp_minus_keys: "tp - len \<in> Mapping.keys a2_map"
+    using a2_map_keys by auto
+  have len_tp: "len \<le> tp"
+    using assms(1) by auto
+  have lin_tss_not_Nil: "linearize tss \<noteq> []"
+    using safe_hd_rep[OF safe_hd_eq] by auto
+  have len_pos: "len > 0"
+    using lin_tss_not_Nil assms(1) by auto
+  have tp_minus_keys': "tp - len + 1 \<in> Mapping.keys a2_map"
+    using a2_map_keys len_pos len_tp by auto
+  obtain m where m_def: "Mapping.lookup a2_map (tp - len) = Some m"
+    using tp_minus_keys by (auto dest: Mapping_keys_dest)
+  obtain m' where m'_def: "Mapping.lookup a2_map (tp - len + 1) = Some m'"
+      using tp_minus_keys' by (auto dest: Mapping_keys_dest)
+  obtain muaux' auxs' done_agg' where updated_def: "(muaux', auxs', done_agg') = eval_step_mmauaux args (?muaux, auxs, done_agg)" by (smt (z3) lin_ts_mmauaux.cases)
+  then obtain tp' tss' len' maskL' maskR' a1_map' a2_map' done' done_length' where split:
+    "muaux' = (tp', tss', len', maskL', maskR', a1_map', a2_map', done', done_length')" using lin_ts_mmuaux.cases by blast
+  have muaux'_def: "muaux' = eval_step_mmuaux args ?muaux" using updated_def m_def safe_hd_eq m'_def by(auto split:option.splits) 
+  have valid_muaux: "valid_mmuaux' args cur dt ?muaux auxlist" using assms(1) by auto
+  have lin_ts_muaux: "lin_ts_mmuaux (tp, tss, len, maskL, maskR, a1_map, a2_map, done, done_length) = ts # tss''" using assms(2) by(auto split:option.splits)
+  have valid_old: "lin_ts_mmauaux (eval_step_mmauaux args ((tp, tss, len, maskL, maskR, a1_map, a2_map, done, done_length), auxs, done_agg)) = tss''"
+                  "valid_mmuaux' args cur dt muaux' auxlist"
+    using updated_def[symmetric] split valid_eval_step_mmuaux'[OF valid_muaux lin_ts_muaux assms(3)] muaux'_def[symmetric]
+    by simp+
+  show ?thesis
+  proof(cases "args_agg args")
+  case None
+  then show ?thesis 
+    using updated_def[symmetric] valid_old split
+    using valid_old by (simp add: muaux'_def)
+  next
+    case aargs: (Some aggargs)
+    then obtain agg_result where done_agg'_def: "done_agg' = agg_result # done_agg" using updated_def m_def safe_hd_eq m'_def by auto
+    let ?m' = "Mapping.filter (\<lambda>_ tstp. ts_tp_lt (args_ivl args) ts (tp - len) tstp) m"
+    have done'_def: "done' = (Mapping.keys ?m')#done" using updated_def split m_def safe_hd_eq aargs m'_def by auto
+    let ?aggaux = "Mapping.lookup auxs (tp - len)"
+    let ?aggaux' = "Mapping.lookup auxs (tp - len + 1)"
+    have subs: "Mapping.keys m - Mapping.keys ?m' \<subseteq> Mapping.keys m" by auto
+    have valid_agg: "valid_maggaux' aggargs ?aggaux (Mapping.keys m)"
+      using assms(1) m_def aargs by(auto simp del: valid_mmuaux'.simps)
+    then have valid_del: "valid_maggaux' aggargs (delete_maggaux' aggargs (Mapping.keys m - Mapping.keys ?m') ?aggaux) (Mapping.keys ?m')"
+    proof(cases ?aggaux)
+      case None
+      then show ?thesis by auto
+    next
+      case (Some a)
+      then have *: "valid_maggaux aggargs a (Mapping.keys m)" using valid_agg by auto
+      then show ?thesis  
+        using valid_delete_maggaux[OF * subs] Some by(auto simp del:delete_maggaux.simps split:prod.splits if_splits) (metis mapping_filter_keys_diff)
+    qed
+    have "agg_result = Some (eval_args_agg args (Mapping.keys ?m')) \<or> agg_result = None"
+    proof(cases "delete_maggaux' aggargs (Mapping.keys m - Mapping.keys ?m') ?aggaux")
+      case None
+      then have "agg_result = None" using done_agg'_def updated_def safe_hd_eq m_def aargs m'_def by auto
+      then show ?thesis by auto
+    next
+      case (Some a)
+      then have *: "valid_maggaux aggargs a (Mapping.keys ?m')" using valid_del by auto
+      have "agg_result = Some (eval_args_agg args (Mapping.keys ?m'))"
+        unfolding eval_args_agg_def using valid_result_maggaux[OF *] aargs done_agg'_def updated_def safe_hd_eq m_def Some m'_def by auto
+      then show ?thesis by auto
+    qed
+    then have valid1: "valid_aggaux_list args done' done_agg'" using done'_def done_agg'_def assms(1) aargs by auto
+    have valid_agg': "valid_maggaux' aggargs ?aggaux' (Mapping.keys m')"
+      using assms(1) m'_def aargs by(auto simp del: valid_mmuaux'.simps)
+    then have *: "valid_maggaux' aggargs (insert_maggaux' aggargs (Mapping.keys ?m' - Mapping.keys m') ?aggaux') (Mapping.keys ?m' \<union> Mapping.keys m')"
+    proof(cases ?aggaux')
+      case None
+      then show ?thesis by auto
+    next
+      case (Some a)
+      then have *: "valid_maggaux aggargs a (Mapping.keys m')" using valid_agg' by auto
+      then show ?thesis  
+        using valid_insert_maggaux[OF *, of "Mapping.keys ?m' - Mapping.keys m'"] Some by(auto simp add: Un_commute simp del:insert_maggaux.simps split:prod.splits)
+    qed
+    then have valid_upd_lookup: "valid_maggaux' aggargs (insert_maggaux' aggargs (Mapping.keys ?m' - Mapping.keys m') (Mapping.lookup auxs (tp - len + 1))) (Mapping.keys (Mapping.combine (\<lambda>tstp tstp'. max_tstp tstp tstp') ?m' m'))" by auto
+    have "\<forall>k m. Mapping.lookup a2_map k = Some m \<longrightarrow> valid_maggaux' aggargs (Mapping.lookup auxs k) (Mapping.keys m)" using assms(1) aargs by auto
+    then have "\<forall>k m. Mapping.lookup a2_map' k = Some m \<longrightarrow> valid_maggaux' aggargs (Mapping.lookup auxs' k) (Mapping.keys m)"
+      using updated_def split aargs safe_hd_eq m_def m'_def assms(1) valid_upd_lookup by(auto simp add:  Mapping_lookup_delete Mapping_lookup_update simp del:valid_mmuaux'.simps insert_maggaux'.simps split:option.splits) 
+    then show ?thesis using updated_def valid_old split aargs safe_hd_eq m_def m'_def valid1 by(auto simp del:valid_mmuaux'.simps)   
+  qed
+qed
+
+lemma valid_eval_step_mmauaux':
+  assumes "valid_mmauaux' args cur dt (mmaux, auxs, done_agg) auxlist"
+    "lin_ts_mmauaux (mmaux, auxs, done_agg) = ts # tss''" "\<not> memR (args_ivl args) (dt - ts)"
+  shows "valid_mmauaux' args cur dt (eval_step_mmauaux args (mmaux, auxs, done_agg)) auxlist \<and>
+    lin_ts_mmauaux (eval_step_mmauaux args (mmaux, auxs, done_agg)) = tss'' \<and> 
+    (case eval_step_mmauaux args (mmaux, auxs, done_agg) of (mmaux', auxs', done_agg') \<Rightarrow>
+    mmaux' = eval_step_mmuaux args mmaux)"
+proof -
+  obtain tp tss len maskL maskR a1_map a2_map donea done_length where "mmaux = (tp, tss, len, maskL, maskR, a1_map, a2_map, donea, done_length)" 
+    using lin_ts_mmuaux.cases by blast
+  then show ?thesis using valid_eval_step_mmauaux_unfolded[of args cur dt tp tss len maskL maskR a1_map a2_map donea done_length auxs done_agg auxlist ts tss'']
+    assms by auto
+qed
+
+lemma valid_foldl_eval_step_mmauaux':
+  assumes valid_before: "valid_mmauaux' args cur dt aux auxlist"
+    "lin_ts_mmauaux aux = tss @ tss'"
+    "\<And>ts. ts \<in> set (take (length tss) (lin_ts_mmauaux aux)) \<Longrightarrow> \<not> memR (args_ivl args) (dt - ts)"
+  shows "valid_mmauaux' args cur dt (foldl (\<lambda>aux _. eval_step_mmauaux args aux) aux tss) auxlist \<and>
+    lin_ts_mmauaux (foldl (\<lambda>aux _. eval_step_mmauaux args aux) aux tss) = tss' \<and> (case (foldl (\<lambda>aux _. eval_step_mmauaux args aux) aux tss) of (mmaux', auxs', done_agg') \<Rightarrow>
+     case aux of (mmaux, auxs, donw_agg) \<Rightarrow> mmaux' = foldl (\<lambda>aux _. eval_step_mmuaux args aux) mmaux tss)"
+  using assms
+proof (induction tss arbitrary: aux)
+  case (Cons ts tss)
+  have app_ass: "lin_ts_mmauaux aux = ts # (tss @ tss')"
+    using Cons(3) by auto
+  obtain mmaux auxs done_agg where split: "aux = (mmaux, auxs, done_agg)" using proj_thd.cases by blast
+  have "\<not> memR (args_ivl args) (dt - ts)"
+    using Cons by auto
+  then have valid_step: "valid_mmauaux' args cur dt (eval_step_mmauaux args aux) auxlist"
+    "lin_ts_mmauaux (eval_step_mmauaux args aux) = tss @ tss'" 
+    "case eval_step_mmauaux args aux of (mmaux', auxs', done_agg') \<Rightarrow>
+     mmaux' = eval_step_mmuaux args mmaux"
+    using valid_eval_step_mmauaux' Cons(2) app_ass split by auto 
+  have *: "\<And>ts. ts \<in> set (take (length tss) (lin_ts_mmauaux (eval_step_mmauaux args aux))) \<Longrightarrow>
+         \<not> memR (args_ivl args) (dt - ts)" using app_ass Cons(4) apply(auto) using valid_step(2) by force
+  have "(case foldl (\<lambda>aux _. eval_step_mmauaux args aux) (eval_step_mmauaux args aux) tss of (mmaux', auxs', done_agg') \<Rightarrow>
+         case eval_step_mmauaux args aux of (mmaux, auxs, donw_agg) \<Rightarrow> 
+         mmaux' = foldl (\<lambda>aux _. eval_step_mmuaux args aux) mmaux tss)"
+    using Cons(1)[OF valid_step(1-2) *] by auto
+  then have "(case foldl (\<lambda>aux _. eval_step_mmauaux args aux) aux (ts # tss) of (mmaux', auxs', done_agg') \<Rightarrow>
+       case aux of (mmaux, auxs, donw_agg) \<Rightarrow> mmaux' = foldl (\<lambda>aux _. eval_step_mmuaux args aux) mmaux (ts # tss))" 
+    using valid_step(3) split by(simp only:foldl.simps split:prod.splits) simp
+  then show ?case
+    using Cons(1)[OF valid_step(1-2)] valid_step Cons(4) app_ass by auto
+qed auto
+
+lemma valid_mmauaux'_mono:
+  assumes "valid_mmauaux' args cur dt aux auxlist" "dt \<le> dt'"
+  shows "valid_mmauaux' args cur dt' aux auxlist"
+  using assms less_le_trans by (cases aux) (fastforce simp: memR_antimono)
+
+
+lemma valid_shift_mmauaux':
+  assumes "valid_mmauaux' args cur cur (mmaux, auxs, done_agg) auxlist" "nt \<ge> cur"
+  shows "valid_mmauaux' args cur nt (shift_mmauaux args nt (mmaux, auxs, done_agg)) auxlist \<and>
+    (\<forall>ts \<in> set (lin_ts_mmauaux (shift_mmauaux args nt (mmaux, auxs, done_agg))). memR (args_ivl args) (nt - ts)) \<and>
+     (case shift_mmauaux args nt (mmaux, auxs, done_agg) of (mmaux', auxs', done_agg') \<Rightarrow> 
+     mmaux' = shift_mmuaux args nt mmaux)"
+proof -
+  define I where "I = args_ivl args"
+  define pos where "pos = args_pos args"
+  let ?aux = "(mmaux, auxs, done_agg)"
+  have valid_folded: "valid_mmauaux' args cur nt ?aux auxlist"
+    using assms(1,2) valid_mmauaux'_mono by blast
+  obtain tp len tss maskL maskR a1_map a2_map "done" done_length where aux_def:
+    "mmaux = (tp, tss, len, maskL, maskR, a1_map, a2_map, done, done_length)"
+    by (cases mmaux) auto
+  note valid_before = valid_folded[unfolded aux_def]
+  define tss_list where "tss_list =
+    linearize (takeWhile_queue (\<lambda>t. \<not> memR I (nt - t)) tss)"
+  have tss_list_takeWhile: "tss_list = takeWhile (\<lambda>t. \<not> memR I (nt - t)) (linearize tss)"
+    using tss_list_def unfolding takeWhile_queue_rep .
+  then obtain tss_list' where tss_list'_def: "linearize tss = tss_list @ tss_list'"
+    "tss_list' = dropWhile (\<lambda>t. \<not> memR I (nt - t)) (linearize tss)"
+    by auto
+  obtain tp' len' tss' maskL' maskR' a1_map' a2_map' "done'" done_length' where
+    foldl_aux_def: "(tp', tss', len', maskL', maskR', a1_map', a2_map',
+      done', done_length') = foldl (\<lambda>aux _. eval_step_mmuaux args aux) mmaux tss_list"
+    by (cases "foldl (\<lambda>aux _. eval_step_mmuaux args aux) mmaux tss_list") auto
+  have lin_tss_aux: "lin_ts_mmauaux (mmaux, auxs, done_agg) = linearize tss"
+    unfolding aux_def by auto
+  have "take (length tss_list) (lin_ts_mmauaux (mmaux, auxs, done_agg)) = tss_list"
+    unfolding lin_tss_aux using tss_list'_def(1) by auto
+  then have valid_foldl: "valid_mmauaux' args cur nt
+    (foldl (\<lambda>aux _. eval_step_mmauaux args aux) (mmaux, auxs, done_agg) tss_list) auxlist"
+    "lin_ts_mmauaux (foldl (\<lambda>aux _. eval_step_mmauaux args aux) (mmaux, auxs, done_agg) tss_list) = tss_list'"
+    "case (foldl (\<lambda>aux _. eval_step_mmauaux args aux) (mmaux, auxs, done_agg) tss_list) of (mmaux', auxs', done_agg') \<Rightarrow>
+     mmaux' = foldl (\<lambda>aux _. eval_step_mmuaux args aux) mmaux tss_list"
+    using valid_foldl_eval_step_mmauaux'[OF valid_before[folded aux_def], unfolded lin_tss_aux,
+      OF tss_list'_def(1)] tss_list_takeWhile set_takeWhileD
+    unfolding lin_tss_aux I_def by fastforce+
+  have shift_mmuaux_eq: "shift_mmauaux args nt (mmaux, auxs, done_agg) = foldl (\<lambda>aux _. eval_step_mmauaux args aux) (mmaux, auxs, done_agg) tss_list"
+    using tss_list_def unfolding aux_def I_def by auto
+  have aux: "(case shift_mmauaux args nt (mmaux, auxs, done_agg) of (mmaux', auxs', done_agg') \<Rightarrow> 
+     mmaux' = shift_mmuaux args nt mmaux)" using valid_foldl(3) by(simp only:aux_def shift_mmauaux.simps Let_def tss_list_def shift_mmuaux.simps I_def) 
+  have "\<And>ts. ts \<in> set tss_list' \<Longrightarrow> memR (args_ivl args) (nt - ts)"
+    using sorted_dropWhile_filter tss_list'_def(2) valid_before unfolding I_def by auto
+  then show ?thesis
+    using valid_foldl(1)[unfolded shift_mmuaux_eq[symmetric]] aux
+    unfolding valid_foldl(2)[unfolded shift_mmuaux_eq[symmetric]] by auto
+qed
+
+lemma upd_nested_agg_lookup: "Mapping.lookup (upd_nested_agg m args ma X) a =
+  (case Mapping.lookup ma a of 
+   Some m' \<Rightarrow> insert_maggaux' args ({b. (a, b) \<in> X} - Mapping.keys m') (Mapping.lookup m a) |
+   None \<Rightarrow> if a \<in> fst ` X then insert_maggaux' args {b. (a, b) \<in> X} (init_maggaux' args) else None)"
+  by (simp add: Mapping.lookup.abs_eq upd_nested_agg.abs_eq)
+
+lemma valid_upd_nested_comb:
+  assumes "\<forall>k m. Mapping.lookup a2_map k = Some m \<longrightarrow> valid_maggaux' aggargs (Mapping.lookup auxs k) (Mapping.keys m)"
+  shows "\<forall>k m. Mapping.lookup (upd_nested a2_map d f X) k = Some m \<longrightarrow> valid_maggaux' aggargs (Mapping.lookup (upd_nested_agg auxs aggargs a2_map X) k) (Mapping.keys m)"
+proof(rule allI, rule allI, rule impI)
+  fix k m
+  assume assm: "Mapping.lookup (upd_nested a2_map d f X) k = Some m"
+  note lookup_map = upd_nested_lookup[of a2_map d f X k] 
+  note lookup_agg = upd_nested_agg_lookup[of auxs aggargs a2_map X k] 
+  show "valid_maggaux' aggargs (Mapping.lookup (upd_nested_agg auxs aggargs a2_map X) k) (Mapping.keys m)"
+  proof(cases "Mapping.lookup a2_map k")
+    case None
+    then show ?thesis 
+    proof(cases "k \<in> fst ` X")
+      case True
+      then have keys: "Mapping.keys m = {b. (k, b) \<in> X}" using assm None lookup_map upd_set'_keys[of _ d f "{b. (k, b) \<in> X}"] by auto
+      have valid_init: "valid_maggaux' aggargs (init_maggaux' aggargs) {}" using valid_init_maggaux by auto
+      have *: "{} \<inter> {b. (k, b) \<in> X} = {}" by simp
+      have "valid_maggaux' aggargs (insert_maggaux' aggargs {b. (k, b) \<in> X} (init_maggaux' aggargs)) {b. (k, b) \<in> X}"
+        using valid_insert_maggaux[OF _ _ *, of aggargs] by(auto simp del:insert_maggaux.simps init_maggaux.simps split:prod.splits) (metis Int_Un_eq(2) case_prodD inf_bot_left valid_init_maggaux)
+      then show ?thesis using lookup_map lookup_agg keys None True
+        by(auto simp del:insert_maggaux.simps init_maggaux'.simps split:option.splits) 
+    next
+      case False 
+      then show ?thesis using assm None lookup_map by auto
+    qed
+  next
+    case m_old: (Some m_old)
+    then have keys: "Mapping.keys m = Mapping.keys m_old \<union> {b. (k, b) \<in> X}" using assm lookup_map upd_set'_keys[of m_old d f "{b. (k, b) \<in> X}"] by auto
+    then show ?thesis 
+    proof(cases "Mapping.lookup auxs k")
+      case None
+      then show ?thesis using lookup_agg m_old by auto
+      next
+        case (Some aux)
+        have *: "Mapping.keys m_old \<inter> ({b. (k, b) \<in> X} - Mapping.keys m_old) = {}" by auto
+        have **: "valid_maggaux aggargs aux (Mapping.keys m_old)" using assms m_old Some by force 
+        have "valid_maggaux' aggargs (insert_maggaux' aggargs ({b. (k, b) \<in> X} - Mapping.keys m_old) (Some aux)) (Mapping.keys m)"
+          using valid_insert_maggaux[OF ** _ *] keys[symmetric] by(auto split:prod.splits)
+        then show ?thesis using m_old lookup_agg Some by auto
+      qed
+  qed
+qed
+
+lemma valid_add_new_mmauaux_unfolded:
+  assumes valid_before: "valid_mmauaux args cur ((tp, tss, len, maskL, maskR, a1_map, a2_map, done, done_length), auxs, done_agg) auxlist"
+    and tabs: "table (args_n args) (args_L args) rel1" "table (args_n args) (args_R args) rel2"
+    and nt_mono: "nt \<ge> cur"
+  shows "valid_mmauaux args nt (add_new_mmauaux args rel1 rel2 nt ((tp, tss, len, maskL, maskR, a1_map, a2_map, done, done_length), auxs, done_agg))
+    (update_until args rel1 rel2 nt auxlist)"
+proof - 
+  let ?muaux = "(tp, tss, len, maskL, maskR, a1_map, a2_map, done, done_length)"
+  have *: "valid_mmauaux' args cur cur (?muaux, auxs, done_agg) auxlist" using valid_before unfolding valid_mmauaux_def by auto
+  obtain muaux' auxs' done_agg' where updated_def: "(muaux', auxs', done_agg') = add_new_mmauaux args rel1 rel2 nt (?muaux, auxs, done_agg)" by (smt (z3) lin_ts_mmauaux.cases)
+  then obtain tp' tss' len' maskL' maskR' a1_map' a2_map' done' done_length' where split:
+    "muaux' = (tp', tss', len', maskL', maskR', a1_map', a2_map', done', done_length')" using lin_ts_mmuaux.cases by blast
+  obtain muaux_i auxs_i done_agg_i where inter_def: "(muaux_i, auxs_i, done_agg_i) = shift_mmauaux args nt (?muaux, auxs, done_agg)" by (smt (z3) lin_ts_mmauaux.cases)
+  then obtain tp_i tss_i len_i maskL_i maskR_i a1_map_i a2_map_i done_i done_length_i where split_i:
+    "muaux_i = (tp_i, tss_i, len_i, maskL_i, maskR_i, a1_map_i, a2_map_i, done_i, done_length_i)" using lin_ts_mmuaux.cases by blast
+  define new_tstp where "new_tstp = (if memL (args_ivl args) 0 then Inr tp_i else Inl nt)"
+  define tmp where "tmp = \<Union>((\<lambda>as. case Mapping.lookup a1_map_i (proj_tuple maskL_i as) of None \<Rightarrow>
+      (if \<not>(args_pos args) then {(tp_i - len_i, as)} else {})
+      | Some tp' \<Rightarrow> if (args_pos args) then {(max (tp_i - len_i) tp', as)}
+      else {(max (tp_i - len_i) (tp' + 1), as)}) ` rel2) \<union> (if memL (args_ivl args) 0 then {tp_i} \<times> rel2 else {})"
+  have shift_lemmas: "muaux_i = shift_mmuaux args nt ?muaux"
+    "valid_mmauaux' args cur nt (muaux_i, auxs_i, done_agg_i) auxlist"
+    using valid_shift_mmauaux'[OF * nt_mono] inter_def by auto
+  have muaux'_def: "muaux' = add_new_mmuaux args rel1 rel2 nt ?muaux" 
+    using updated_def inter_def[symmetric] split[symmetric] shift_lemmas(1) by(auto simp del:shift_mmauaux.simps shift_mmuaux.simps split:option.splits prod.splits)
+  have valid_old: "valid_mmuaux args cur ?muaux auxlist" using assms(1) unfolding valid_mmauaux_def valid_mmuaux_def by auto
+  have valid_muaux: "valid_mmuaux args nt muaux' (update_until args rel1 rel2 nt auxlist)" 
+    using valid_add_new_mmuaux[OF valid_old tabs nt_mono] muaux'_def by simp
+  show ?thesis
+  proof(cases "args_agg args")
+    case None
+    then show ?thesis using valid_muaux unfolding updated_def[symmetric] valid_mmauaux_def split valid_mmauaux'.simps valid_mmuaux_def by auto
+  next
+    case (Some aggargs)
+    have upd_defs: "a2_map' = Mapping.update (tp_i + 1) Mapping.empty (upd_nested a2_map_i new_tstp (max_tstp new_tstp) tmp)"
+         "auxs' = (let auxs'' = upd_nested_agg auxs_i aggargs a2_map_i tmp in
+          case init_maggaux' aggargs of None \<Rightarrow> auxs'' |
+          Some aux \<Rightarrow> Mapping.update (tp_i + 1) aux auxs'')"
+          "done' = done_i" "done_agg' = done_agg_i"
+      using Some updated_def unfolding tmp_def new_tstp_def add_new_mmauaux.simps unfolding inter_def[symmetric] split_i split by(auto)
+    have *: "\<forall>k m. Mapping.lookup a2_map_i k = Some m \<longrightarrow> valid_maggaux' aggargs (Mapping.lookup auxs_i k) (Mapping.keys m)"
+            "valid_aggaux_list args done_i done_agg_i"
+      using shift_lemmas(2) Some split_i by auto
+    note inter_valid =  valid_upd_nested_comb[OF *(1), of new_tstp "max_tstp new_tstp" tmp]
+    have "valid_maggaux' aggargs (init_maggaux' aggargs) {}" using valid_init_maggaux by auto
+    then have "\<forall>k m. Mapping.lookup a2_map' k = Some m \<longrightarrow> valid_maggaux' aggargs (Mapping.lookup auxs' k) (Mapping.keys m)"
+      using upd_defs inter_valid Mapping.lookup_update'[of "(Suc tp_i)" "Mapping.empty" "(upd_nested a2_map_i new_tstp (max_tstp new_tstp) tmp)"]
+        Mapping.lookup_update'[of "(Suc tp_i)" _ "upd_nested_agg auxs_i aggargs a2_map_i tmp"]
+      by(auto simp add:lookup_update  simp del:init_maggaux.simps split:prod.splits) simp
+    then show ?thesis using valid_muaux *(2) unfolding updated_def[symmetric] valid_mmauaux_def split valid_mmauaux'.simps upd_defs(3-4) valid_mmuaux_def Some 
+      by(simp del:valid_mmuaux'.simps) 
+  qed
+qed
+
+lemma valid_add_new_mmauaux:
+  assumes valid_before: "valid_mmauaux args cur (mmaux, auxs, done_agg) auxlist"
+    and tabs: "table (args_n args) (args_L args) rel1" "table (args_n args) (args_R args) rel2"
+    and nt_mono: "nt \<ge> cur"
+  shows "valid_mmauaux args nt (add_new_mmauaux args rel1 rel2 nt (mmaux, auxs, done_agg))
+    (update_until args rel1 rel2 nt auxlist)"
+  using valid_add_new_mmauaux_unfolded[OF _ tabs nt_mono] valid_before by (cases mmaux) fast
+
+lemma done_empty_valid_mmauaux'_intro:
+  assumes "valid_mmauaux' args cur dt
+    ((tp, tss, len, maskL, maskR, a1_map, a2_map, done, done_length), auxs, done_agg) auxlist"
+  shows "valid_mmauaux' args cur dt'
+    ((tp, tss, len, maskL, maskR, a1_map, a2_map, [], 0), auxs, [])
+    (drop (length done) auxlist)"
+  using assms sorted_drop by (auto simp add: drop_map[symmetric] split:option.splits)
+
+lemma valid_agg_list_rev:
+  assumes "valid_aggaux_list args done done_agg"
+  shows "valid_aggaux_list args (rev done) (rev done_agg)"
+  sorry
+
+lemma valid_eval_mmauaux:
+  assumes "valid_mmauaux args cur (mmaux, auxs, done_agg) auxlist" "nt \<ge> cur"
+    "eval_mmauaux args nt (mmaux, auxs, done_agg) = (res, res_agg, aux')" "eval_until (args_ivl args) nt auxlist = (res', auxlist')"
+  shows "res = res' \<and> valid_mmauaux args cur aux' auxlist' \<and> (case args_agg args of Some aggargs \<Rightarrow> valid_aggaux_list args res res_agg|
+                                                                                    None \<Rightarrow> True)"
+proof -
+  define I where "I = args_ivl args"
+  define pos where "pos = args_pos args"
+  have valid_folded: "valid_mmauaux' args cur nt (mmaux, auxs, done_agg) auxlist"
+    using assms(1,2) valid_mmauaux'_mono unfolding valid_mmauaux_def by blast
+  obtain tp len tss maskL maskR a1_map a2_map "done" done_length auxs' done_agg' where shift_aux_def:
+    "shift_mmauaux args nt (mmaux, auxs, done_agg) = ((tp, tss, len, maskL, maskR, a1_map, a2_map, done, done_length), auxs', done_agg')"
+    by (cases "shift_mmauaux args nt (mmaux, auxs, done_agg)") auto
+  have valid_shift_aux: "valid_mmauaux' args cur nt ((tp, tss, len, maskL, maskR,
+    a1_map, a2_map, done, done_length), auxs', done_agg') auxlist"
+    "\<And>ts. ts \<in> set (linearize tss) \<Longrightarrow> memR (args_ivl args) (nt - ts)"
+    using valid_shift_mmauaux'[OF assms(1)[unfolded valid_mmauaux_def]  assms(2)]
+    unfolding shift_aux_def by auto
+  have len_done_auxlist: "length done \<le> length auxlist"
+    using valid_shift_aux by auto
+  have list_all: "\<And>x. x \<in> set (take (length done) auxlist) \<Longrightarrow> check_before I nt x"
+    using valid_shift_aux unfolding I_def by auto
+  have set_drop_auxlist: "\<And>x. x \<in> set (drop (length done) auxlist) \<Longrightarrow> \<not>check_before I nt x"
+    using valid_shift_aux[unfolded valid_mmauaux'.simps valid_mmuaux'.simps]
+      list_all2_check_before[OF _ valid_shift_aux(2)] unfolding I_def by fast
+  have take_auxlist_takeWhile: "take (length done) auxlist = takeWhile (check_before I nt) auxlist"
+    using len_done_auxlist list_all set_drop_auxlist
+    by (rule take_takeWhile) assumption+
+  have rev_done: "rev done = map proj_thd (take (length done) auxlist)"
+    using valid_shift_aux by auto
+  then have res'_def: "res' = rev done"
+    using eval_until_res[OF assms(4)] unfolding take_auxlist_takeWhile I_def by auto
+  then have auxlist'_def: "auxlist' = drop (length done) auxlist"
+    using eval_until_auxlist'[OF assms(4)] by auto
+  have eval_mmuaux_eq: "eval_mmauaux args nt (mmaux, auxs, done_agg)  = (rev done, rev done_agg', ((tp, tss, len, maskL, maskR,
+    a1_map, a2_map, [], 0), auxs', []))"
+    using shift_aux_def by auto
+  have "case args_agg args of Some aggargs \<Rightarrow> valid_aggaux_list args done done_agg' |
+                              None \<Rightarrow> True" using valid_shift_aux(1) unfolding valid_mmauaux'.simps
+    by(auto split:option.splits)
+  then have "case args_agg args of Some aggargs \<Rightarrow> valid_aggaux_list args (rev done) (rev done_agg') |
+                              None \<Rightarrow> True"
+    using valid_agg_list_rev[of args "done" done_agg'] by(auto split:option.splits)
+  then show ?thesis
+    using assms(3) done_empty_valid_mmauaux'_intro[OF valid_shift_aux(1)]
+    unfolding shift_aux_def eval_mmuaux_eq pos_def auxlist'_def res'_def valid_mmauaux_def by (auto simp del:valid_mmuaux'.simps split:option.splits)
+qed
+
+lemma valid_eval_mmauaux':
+  assumes "valid_mmauaux args cur (mmaux, auxs, done_agg) auxlist" "nt \<ge> cur"
+    "eval_mmauaux' args nt (mmaux, auxs, done_agg) = (res,  aux')" "eval_until (args_ivl args) nt auxlist = (res', auxlist')"
+  shows "valid_mmauaux args cur aux' auxlist' \<and> res = map (eval_args_agg args) res'"
+  using assms(3) valid_eval_mmauaux[OF assms(1-2) _ assms(4)]
+  sorry
+
+interpretation default_mmauaux: muaux valid_mmauaux init_mmauaux add_new_mmauaux length_mmauaux eval_mmauaux'
+  using valid_init_mmauaux valid_add_new_mmauaux valid_length_mmauaux valid_eval_mmauaux'
   by unfold_locales (auto split:prod.splits)
 
 end
